common/MemoryC.v
@@ -603,4 +603,266 @@ Proof.
   eapply prop_ext4. eapply Mem_store_perm_iff; eauto.
 Qed.
 
+Local Transparent store.
+Lemma Mem_store_mapped_inject_undef
+      f m1 m2 b1 ofs chunk n1
+      (INJ: Mem.inject f m1 m2)
+      (STORESRC: Mem.store chunk m1 b1 ofs Vundef = Some n1)
+  :
+    inject f n1 m2
+.
+Proof.
+  hexploit Mem_store_perm_iff; eauto. intro PERM. des.
+  econs; try apply INJ; eauto.
+  - econs; eauto.
+    + ii; clarify. eapply INJ; eauto. eapply PERM; eauto.
+    + ii; clarify. eapply INJ; eauto. ii. eapply PERM; eauto.
+    + ii; clarify.
+      unfold store in *. des_ifs. ss.
+      unfold ZMap.get; rewrite PMap.gsspec. des_ifs; cycle 1.
+      { eapply INJ; eauto. }
+      unfold perm in *. ss.
+      (* inv INJ. clear_until mi_inj0. inv mi_inj0. clear mi_perm0 mi_align0. *)
+      destruct chunk; ss; repeat (unfold ZMap.set in *; rewrite PMap.gsspec; des_ifs; [econs; eauto|]);
+        eapply INJ; eauto.
+ - admit "ez".
+ - admit "ez".
+ - admit "ez".
+ - admit "ez".
+Qed.
+
 End ARGPASSING.
+
+Section STORED.
+
+
+Inductive Mem_stored (chunk: memory_chunk) (m0: mem) (b: block) (ofs: Z) (v: val): Prop :=
+| stored_intro
+    (STORED: (Mem.getN (size_chunk_nat chunk) ofs (Maps.PMap.get b m0.(Mem.mem_contents)))
+             = (encode_val chunk v))
+    (WRITABLE: Mem.valid_access m0 chunk b ofs Writable)
+.
+
+Definition Mem_storedv chunk m addr v: Prop :=
+  match addr with
+  | Vptr b ofs true => Mem_stored chunk m b (Ptrofs.unsigned ofs) v
+  | _ => False
+  end
+.
+
+Theorem Mem_store_stored
+        chunk m0 b ofs v m1
+        (STORE: Mem.store chunk m0 b ofs v = Some m1)
+  :
+    <<STORED: Mem_stored chunk m1 b ofs v>>
+.
+Proof.
+  econs; eauto with mem.
+  erewrite Mem.store_mem_contents; eauto.
+  rewrite Maps.PMap.gsspec. des_ifs.
+  erewrite <- encode_val_length; eauto.
+  rewrite Mem.getN_setN_same. ss.
+Qed.
+
+(* Local Transparent Mem.load. *)
+(* Lemma Mem_stored_load *)
+(*       chunk m0 b ofs v *)
+(*       (STORE: Mem_stored chunk m0 b ofs v) *)
+(*   : *)
+(*     <<LOAD: Mem.load chunk m0 b ofs = Some v>> *)
+(* . *)
+(* Proof. *)
+(*   inv STORE. *)
+(*   unfold Mem.load. des_ifs; cycle 1. *)
+(*   { exfalso. eapply n. eauto with mem. } *)
+(*   red. f_equal. *)
+(*   destruct chunk; ss; des_ifs. *)
+(*   - unfold encode_val in *. *)
+(*   destruct chunk; ss. *)
+(*   - unfold Maps.PMap.get. des_ifs. econs; eauto. *)
+(* Qed. *)
+(* Local Opaque Mem.load. *)
+
+(* Local Transparent Mem.store. *)
+
+(* Definition ZMap_equal {X} (eqX: X -> X -> Prop) (EQUIV: RelationClasses.Equivalence eqX) *)
+(*            (zm0 zm1: Maps.ZMap.t X): Prop := *)
+(*   zm0.(fst) = zm1.(fst) /\ Maps.PTree_Properties.Equal EQUIV zm0.(snd) zm1.(snd) *)
+(* . *)
+
+(* Inductive Mem_equal (m0 m1: mem): Prop := *)
+(* | equal_intro *)
+(*       (EQ0: m0.(Mem.mem_contents).(fst) = m1.(Mem.mem_contents).(fst)) *)
+(*       (EQ1: @Maps.PTree_Properties.Equal _ (ZMap_equal eq (@Eqsth _)) *)
+(*                                          (admit "") *)
+(*                                          m0.(Mem.mem_contents).(snd) m1.(Mem.mem_contents).(snd)) *)
+(*       (EQ2: m0.(Mem.mem_access) = m1.(Mem.mem_access)) *)
+(*       (EQ3: m0.(Mem.nextblock) = m1.(Mem.nextblock)) *)
+(* . *)
+
+(* Theorem Mem_stored_store *)
+(*         chunk m0 b ofs v *)
+(*         (STORED: Mem_stored chunk m0 b ofs v) *)
+(*   : *)
+(*     exists m1, <<STORE: Mem.store chunk m0 b ofs v = Some m1>> /\ *)
+(*                         <<EQUIV: Mem_equal m0 m1>> *)
+(* . *)
+(* Proof. *)
+(*   inv STORED. *)
+(*   unfold Mem.store. des_ifs. destruct m0; ss. *)
+(*   esplits; eauto. *)
+(*   econs; eauto. cbn. *)
+(*   destruct mem_contents; ss. *)
+(*   hnf. ii; ss. *)
+(*   destruct (Maps.PTree.get x t0) eqn:T. *)
+(*   - rewrite Maps.PTree.gsspec. rewrite T. *)
+(*     unfold Maps.PMap.get in *. ss. des_ifs; try reflexivity. *)
+(*     econs; ss. *)
+(*     { rewrite Mem.setN_default. ss. } *)
+(*     hnf. ii. *)
+(*     destruct (Maps.PTree.get x (snd t1)) eqn:U. *)
+(*     + *)
+(*     des_ifs. *)
+(*     rewrite <- STORED0. erewrite <- encode_val_length with (v:=v); eauto. *)
+(*     rewrite Mem.getN_setN_same. ss. *)
+(*     econs; eauto. *)
+(*   unfold Maps.PMap.set. ss. f_equal. *)
+(*   Maps.PTree_Properties.Equal *)
+(*   assert(forall i, Maps.PTree.set b (Mem.setN (encode_val chunk v) ofs (Maps.PMap.get b (t, t0))) t0 *)
+(*   rewrite Maps.PTree.gsspec. *)
+(*   eapply Axioms.functional_extensionality. *)
+(*   cbn. *)
+(*   Set Printing All. *)
+(*   rewrite Maps.PMap.gsspec. *)
+(*   rewrite Mem.getN_setN_same. ss. *)
+(*   econs; eauto. *)
+(*   econs; eauto with mem. *)
+(*   erewrite Mem.store_mem_contents; eauto. *)
+(*   rewrite Maps.PMap.gsspec. des_ifs. *)
+(*   erewrite <- encode_val_length; eauto. *)
+(*   rewrite Mem.getN_setN_same. ss. *)
+(* Qed. *)
+
+
+(* Lemma Mem_equal_proof_irr *)
+(*       m0 m1 *)
+(*       (EQ0: m0.(Mem.mem_contents) = m1.(Mem.mem_contents)) *)
+(*       (EQ1: m0.(Mem.mem_access) = m1.(Mem.mem_access)) *)
+(*       (EQ2: m0.(Mem.nextblock) = m1.(Mem.nextblock)) *)
+(*   : *)
+(*     m0 = m1 *)
+(* . *)
+(* Proof. *)
+(*   destruct m0, m1; ss. clarify. *)
+(*   f_equal; eapply Axioms.proof_irr. *)
+(* Qed. *)
+
+(* Theorem Mem_stored_store *)
+(*         chunk m0 b ofs v *)
+(*         (STORED: Mem_stored chunk m0 b ofs v) *)
+(*   : *)
+(*     exists m1, <<STORE: Mem.store chunk m0 b ofs v = Some m1>> /\ *)
+(*                         <<EQUIV: m0 = m1>> *)
+(* . *)
+(* Proof. *)
+(*   inv STORED. *)
+(*   unfold Mem.store. des_ifs. destruct m0; ss. *)
+(*   esplits; eauto. cbn. *)
+(*   f_equal. eapply Mem_equal_proof_irr; eauto. *)
+(*   ss. *)
+(*   destruct mem_contents; ss. *)
+(*   unfold Maps.PMap.set. ss. f_equal. *)
+(*   Maps.PTree_Properties.Equal *)
+(*   assert(forall i, Maps.PTree.set b (Mem.setN (encode_val chunk v) ofs (Maps.PMap.get b (t, t0))) t0 *)
+(*   rewrite Maps.PTree.gsspec. *)
+(*   eapply Axioms.functional_extensionality. *)
+(*   cbn. *)
+(*   Set Printing All. *)
+(*   rewrite Maps.PMap.gsspec. *)
+(*   rewrite Mem.getN_setN_same. ss. *)
+(*   econs; eauto. *)
+(*   econs; eauto with mem. *)
+(*   erewrite Mem.store_mem_contents; eauto. *)
+(*   rewrite Maps.PMap.gsspec. des_ifs. *)
+(*   erewrite <- encode_val_length; eauto. *)
+(*   rewrite Mem.getN_setN_same. ss. *)
+(* Qed. *)
+
+
+Local Existing Instance Val.mi_normal.
+
+Lemma memval_inject_refl
+      mv
+  : 
+    memval_inject (fun b0 : block => Some (b0, 0)) mv mv
+.
+Proof.
+  destruct mv; ss; econs; eauto.
+  apply val_inject_id. ss. 
+Qed.
+
+Lemma store_stored_inject
+      j0 m_src0 m_src1 m_tgt
+      (INJ: Mem.inject j0 m_src0 m_tgt)
+      v_src v_tgt
+      (INJV: Val.inject j0 v_src v_tgt) 
+      ty rsp_src rsp_tgt rspdelta ofs
+      (SRC: Mem.storev (chunk_of_type ty) m_src0 (Vptr rsp_src ofs true) v_src = Some m_src1)
+      (TGT: Mem_stored (chunk_of_type ty) m_tgt rsp_tgt (Ptrofs.unsigned (Ptrofs.add ofs rspdelta)) v_tgt)
+      (INJRSP: j0 rsp_src = Some (rsp_tgt, rspdelta.(Ptrofs.unsigned)))
+      (BOUND: Ptrofs.unsigned ofs + Ptrofs.unsigned rspdelta <= Ptrofs.max_unsigned)
+  :
+    <<INJ: Mem.inject j0 m_src1 m_tgt>>
+.
+Proof.
+  ss. red.
+  exploit Mem.store_mapped_inject; eauto. i; des.
+  eapply Mem.inject_extends_compose; eauto.
+  clear - TGT H BOUND.
+Local Transparent Mem.store.
+  hexploit MemoryC.Mem_store_perm_eq; eauto. intro PERM. des.
+  replace (Ptrofs.unsigned (Ptrofs.add ofs rspdelta)) with
+      (Ptrofs.unsigned ofs + Ptrofs.unsigned rspdelta) in *; cycle 1.
+  { rewrite Ptrofs.add_unsigned. rewrite Ptrofs.unsigned_repr; ss. split; try xomega.
+    hexploit (Ptrofs.unsigned_range ofs); eauto. i.
+    hexploit (Ptrofs.unsigned_range rspdelta); eauto. i.
+    xomega.
+  }
+  abstr (Ptrofs.unsigned ofs + Ptrofs.unsigned rspdelta) ofs0.
+  unfold Mem.store in *. inv TGT. des_ifs.
+  econs; eauto.
+  unfold inject_id.
+  econs; ss; eauto.
+  - ii; clarify. unfold Mem.perm in *; ss. rewrite Z.add_0_r. ss.
+  - ii; clarify. unfold Mem.range_perm, Mem.perm in *. ss. rewrite Z.divide_0_r. reflexivity.
+  - ii; clarify. unfold Mem.perm in *; ss. rewrite Z.add_0_r. ss.
+    rewrite Maps.PMap.gsspec. des_ifs; cycle 1.
+    { apply memval_inject_refl. }
+    rewrite <- STORED.
+    rename rsp_tgt into b. abstr (chunk_of_type ty) chunk. clear_tac.
+    destruct chunk; ss; rewrite ! Maps.ZMap.gsspec; des_ifs; try apply memval_inject_refl.
+Qed.
+
+Lemma Mem_stored_unchanged_on
+      P m0 m1
+      (UNCH: Mem.unchanged_on P m0 m1)
+      b ofs v chunk
+      (INSIDE: forall i : Z, ofs <= i < ofs + size_chunk chunk -> P b i)
+      (STORED: Mem_stored chunk m0 b ofs v)
+  :
+    <<STORED: Mem_stored chunk m1 b ofs v>>
+.
+Proof.
+  inv UNCH.
+  inv STORED. econs; eauto.
+  - erewrite <- STORED0.
+    unfold Mem.valid_access in *. ss. des; ss.
+    apply Mem.range_perm_implies with (p2:= Readable) in WRITABLE; eauto with mem.
+    destruct chunk; ss; rewrite ! unchanged_on_contents; eauto with lia.
+  - hnf in WRITABLE. des.
+    hnf. splits; eauto. ii. eapply unchanged_on_perm; eauto.
+    eauto with mem.
+Qed.
+
+End STORED.
+
